The Leap of Faith

theories/program_logic/adequacy.v
@@ -34,77 +34,78 @@ Proof.
 Qed.
 
 (* Program logic adequacy *)
-Record adequate {Λ} (e1 : expr Λ) (l1: local_state Λ) (σ1 : state Λ) (φ : val Λ → Prop) := {
-  adequate_result t2 l2 σ2 v2 :
-   rtc step ([(e1, l1)], σ1) ((of_val v2, l2) :: t2, σ2) → φ v2;
-  adequate_safe t2 σ2 e2 l2 :
-   rtc step ([(e1, l1)], σ1) (t2, σ2) →
+Record adequate {Λ} (e1 : expr Λ * local_state Λ) (σ1 : state Λ) (φ : val Λ → Prop) := {
+  adequate_result l2 t2 σ2 v2 :
+   rtc step ([e1], σ1) ((of_val v2, l2) :: t2, σ2) → φ v2;
+  adequate_safe l2 t2 σ2 e2 :
+   rtc step ([e1], σ1) (t2, σ2) →
    (e2, l2) ∈ t2 → (is_Some (to_val e2) ∨ reducible e2 l2 σ2)
 }.
 
-Theorem adequate_tp_safe {Λ} (e1 : expr Λ) l1 t2 σ1 σ2 φ :
-  adequate e1 l1 σ1 φ →
-  rtc step ([(e1, l1)], σ1) (t2, σ2) →
+Theorem adequate_tp_safe {Λ} (e1 : expr Λ * local_state Λ) t2 σ1 σ2 φ :
+  adequate e1 σ1 φ →
+  rtc step ([e1], σ1) (t2, σ2) →
   Forall (λ e, is_Some (to_val (e.1))) t2 ∨ ∃ t3 σ3, step (t2, σ2) (t3, σ3).
 Proof.
   intros Had ?.
   destruct (decide (Forall (λ e, is_Some (to_val (e.1))) t2)) as [|Ht2]; [by left|].
-  apply (not_Forall_Exists _), Exists_exists in Ht2; destruct Ht2 as ((e2&l2)&?&He2).
-  destruct (adequate_safe e1 l1 σ1 φ Had t2 σ2 e2 l2) as [?|(e3&l3&σ3&efs&?)];
+  apply (not_Forall_Exists _), Exists_exists in Ht2; destruct Ht2 as (e2&?&He2).
+  destruct e2 as [e2 l2].
+  destruct (adequate_safe e1 σ1 φ Had l2 t2 σ2 e2) as [?|(e3&l3&σ3&efs&?)];
     rewrite ?eq_None_not_Some; auto.
   { exfalso. eauto. }
   destruct (elem_of_list_split t2 (e2, l2)) as (t2'&t2''&->); auto.
-  right; exists (t2' ++ (e3, l3) :: t2'' ++ (map (,init_local Λ) efs)), σ3; econstructor; eauto.
+  right; exists (t2' ++ (e3, l3) :: t2'' ++ map (,init_local Λ) efs), σ3; econstructor; eauto.
 Qed.
 
 Section adequacy.
 Context `{irisG Λ Σ}.
-Implicit Types e : expr Λ.
+Implicit Types e : expr Λ * local_state Λ.
 Implicit Types P Q : iProp Σ.
 Implicit Types Φ : val Λ → iProp Σ.
 Implicit Types Φs : list (val Λ → iProp Σ).
 
 Notation world σ := (wsat ∗ ownE ⊤ ∗ state_interp σ)%I.
 
-Notation wptp t := ([∗ list] ef ∈ t, WP (ef.1) {{ _, True }})%I.
+Notation wptp t := ([∗ list] ef ∈ t, WP ef {{ _, True }})%I.
 
-Lemma wp_step e1 l1 σ1 e2 l2 σ2 efs Φ :
-  prim_step e1 l1 σ1 e2 l2 σ2 efs →
-  world σ1 ∗ WP e1 {{ Φ }} ==∗ ▷ |==> ◇ (world σ2 ∗ WP e2 {{ Φ }} ∗ wptp (map (,init_local Λ) efs)).
+Lemma wp_step e1 σ1 e2 σ2 efs Φ :
+  prim_step (e1.1) (e1.2) σ1 (e2.1) (e2.2) σ2 efs →
+  world σ1 ∗ WP e1 {{ Φ }} ==∗ ▷ |==> ◇ (world σ2 ∗ WP e2 {{ Φ }} ∗ wptp (map (, init_local Λ) efs)).
 Proof.
   rewrite {1}wp_unfold /wp_pre. iIntros (Hstep) "[(Hw & HE & Hσ) [H|[_ H]]]".
   { iDestruct "H" as (v) "[% _]". apply val_stuck in Hstep; simplify_eq. }
   rewrite fupd_eq /fupd_def.
-  iMod ("H" $! l1 σ1 with "Hσ [Hw HE]") as ">(Hw & HE & _ & H)"; first by iFrame.
+  iMod ("H" $! σ1 with "Hσ [Hw HE]") as ">(Hw & HE & _ & H)"; first by iFrame.
   iModIntro; iNext.
-  iMod ("H" $! e2 l2 σ2 efs with "[%] [$Hw $HE]") as ">($ & $ & $ & $ & ?)"=>//.
-Admitted. (* apparent ... *)
+  (* by iMod ("H" $! e2 σ2 efs with "[%] [$Hw $HE]") as ">($ & $ & $ & $)". *)
+Admitted.
 
-Lemma wptp_step e1 l1 t1 t2 σ1 σ2 Φ :
-  step ((e1, l1) :: t1,σ1) (t2, σ2) →
+Lemma wptp_step e1 t1 t2 σ1 σ2 Φ :
+  step (e1 :: t1,σ1) (t2, σ2) →
   world σ1 ∗ WP e1 {{ Φ }} ∗ wptp t1
-  ==∗ ∃ e2 l2 t2', ⌜t2 = (e2, l2) :: t2'⌝ ∗ ▷ |==> ◇ (world σ2 ∗ WP e2 {{ Φ }} ∗ wptp t2').
+  ==∗ ∃ e2 t2', ⌜t2 = e2 :: t2'⌝ ∗ ▷ |==> ◇ (world σ2 ∗ WP e2 {{ Φ }} ∗ wptp t2').
 Proof.
   iIntros (Hstep) "(HW & He & Ht)".
   destruct Hstep as [e1' l1' σ1' e2' l2' σ2' efs [|? t1'] t2' ?? Hstep]; simplify_eq/=.
-  - iExists e2', l2', (t2' ++ map (,init_local Λ) efs); iSplitR; first eauto.
+  - iExists (e2', l2'), (t2' ++ map (,init_local Λ) efs); iSplitR; first eauto.
     rewrite big_sepL_app. iFrame "Ht". iApply wp_step; try iFrame; eauto.
-  - iExists e1, l1, (t1' ++ (e2', l2') :: t2' ++ map (,init_local Λ) efs); iSplitR; first eauto.
+  - iExists p, (t1' ++ (e2', l2') :: t2' ++ map (,init_local Λ) efs); iSplitR; first eauto.
     rewrite !big_sepL_app !big_sepL_cons big_sepL_app.
-    iDestruct "Ht" as "($ & He' & $)"; iFrame "He". simpl.
+    iDestruct "Ht" as "($ & He' & $)"; iFrame "He".
     iApply wp_step; try iFrame; eauto.
 Qed.
 
-Lemma wptp_steps n e1 l1 t1 t2 σ1 σ2 Φ :
-  nsteps step n ((e1, l1) :: t1, σ1) (t2, σ2) →
+Lemma wptp_steps n e1 t1 t2 σ1 σ2 Φ :
+  nsteps step n (e1 :: t1, σ1) (t2, σ2) →
   world σ1 ∗ WP e1 {{ Φ }} ∗ wptp t1 ⊢
-  Nat.iter (S n) (λ P, |==> ▷ P) (∃ e2 l2 t2',
-    ⌜t2 = (e2, l2) :: t2'⌝ ∗ world σ2 ∗ WP e2 {{ Φ }} ∗ wptp t2').
+  Nat.iter (S n) (λ P, |==> ▷ P) (∃ e2 t2',
+    ⌜t2 = e2 :: t2'⌝ ∗ world σ2 ∗ WP e2 {{ Φ }} ∗ wptp t2').
 Proof.
-  revert e1 l1 t1 t2 σ1 σ2; simpl; induction n as [|n IH]=> e1 l1 t1 t2 σ1 σ2 /=.
+  revert e1 t1 t2 σ1 σ2; simpl; induction n as [|n IH]=> e1 t1 t2 σ1 σ2 /=.
   { inversion_clear 1; iIntros "?"; eauto 10. }
   iIntros (Hsteps) "H". inversion_clear Hsteps as [|?? [t1' σ1']].
-  iMod (wptp_step with "H") as (e1' l1' t1'') "[% H]"; first eauto; simplify_eq.
+  iMod (wptp_step with "H") as (e1' t1'') "[% H]"; first eauto; simplify_eq.
   iModIntro; iNext; iMod "H" as ">?". by iApply IH.
 Qed.
 
@@ -118,20 +119,20 @@ Proof.
   by rewrite bupd_frame_l {1}(later_intro R) -later_sep IH.
 Qed.
 
-Lemma wptp_result n e1 l1 l2 t1 v2 t2 σ1 σ2 φ :
-  nsteps step n ((e1, l1) :: t1, σ1) ((of_val v2, l2) :: t2, σ2) →
+Lemma wptp_result n e1 t1 v2 t2 σ1 σ2 l2 φ :
+  nsteps step n (e1 :: t1, σ1) ((of_val v2, l2) :: t2, σ2) →
   world σ1 ∗ WP e1 {{ v, ⌜φ v⌝ }} ∗ wptp t1 ⊢
   Nat.iter (S (S n)) (λ P, |==> ▷ P) ⌜φ v2⌝.
 Proof.
   intros. rewrite wptp_steps //.
   rewrite (Nat_iter_S_r (S n)). apply bupd_iter_mono.
-  iDestruct 1 as (e2 l2' t2') "(% & (Hw & HE & _) & H & _)"; simplify_eq.
+  iDestruct 1 as (e2 t2') "(% & (Hw & HE & _) & H & _)"; simplify_eq.
   iDestruct (wp_value_inv with "H") as "H". rewrite fupd_eq /fupd_def.
   iMod ("H" with "[Hw HE]") as ">(_ & _ & $)"; iFrame; auto.
 Qed.
 
-Lemma wp_safe e l σ Φ :
-  world σ ∗ WP e {{ Φ }} ==∗ ▷ ⌜is_Some (to_val e) ∨ reducible e l σ⌝.
+Lemma wp_safe e σ Φ :
+  world σ ∗ WP e {{ Φ }} ==∗ ▷ ⌜is_Some (to_val (e.1)) ∨ reducible (e.1) (e.2) σ⌝.
 Proof.
   rewrite wp_unfold /wp_pre. iIntros "[(Hw&HE&Hσ) [H|[_ H]]]".
   { iDestruct "H" as (v) "[% _]"; eauto 10. }
@@ -139,69 +140,68 @@ Proof.
   eauto 10.
 Qed.
 
-Lemma wptp_safe n e1 l1 e2 l2 t1 t2 σ1 σ2 Φ :
-  nsteps step n ((e1, l1) :: t1, σ1) (t2, σ2) → (e2, l2) ∈ t2 →
+Lemma wptp_safe n e1 e2 t1 t2 σ1 σ2 Φ :
+  nsteps step n (e1 :: t1, σ1) (t2, σ2) → e2 ∈ t2 →
   world σ1 ∗ WP e1 {{ Φ }} ∗ wptp t1 ⊢
-  Nat.iter (S (S n)) (λ P, |==> ▷ P) ⌜is_Some (to_val e2) ∨ reducible e2 l2 σ2⌝.
+  Nat.iter (S (S n)) (λ P, |==> ▷ P) ⌜is_Some (to_val (e2.1)) ∨ reducible (e2.1) (e2.2) σ2⌝.
 Proof.
   intros ? He2. rewrite wptp_steps //; rewrite (Nat_iter_S_r (S n)). apply bupd_iter_mono.
-  iDestruct 1 as (e2' l2' t2') "(% & Hw & H & Htp)"; simplify_eq.
-  apply elem_of_cons in He2 as [?|?]; first (inversion H0; subst; iApply wp_safe; by iFrame "Hw H").
-  iApply wp_safe. iFrame "Hw".
-  (* iApply (big_sepL_elem_of with "Htp"). *)
-Admitted.
+  iDestruct 1 as (e2' t2') "(% & Hw & H & Htp)"; simplify_eq.
+  apply elem_of_cons in He2 as [<-|?]; first (iApply wp_safe; by iFrame "Hw H").
+  iApply wp_safe. iFrame "Hw". by iApply (big_sepL_elem_of with "Htp").
+Qed.
 
-Lemma wptp_invariance n e1 l1 e2 t1 t2 σ1 σ2 φ Φ :
-  nsteps step n ((e1, l1) :: t1, σ1) (t2, σ2) →
+Lemma wptp_invariance n e1 e2 t1 t2 σ1 σ2 φ Φ :
+  nsteps step n (e1 :: t1, σ1) (t2, σ2) →
   (state_interp σ2 ={⊤,∅}=∗ ⌜φ⌝) ∗ world σ1 ∗ WP e1 {{ Φ }} ∗ wptp t1
   ⊢ Nat.iter (S (S n)) (λ P, |==> ▷ P) ⌜φ⌝.
 Proof.
   intros ?. rewrite wptp_steps //.
   rewrite (Nat_iter_S_r (S n)) !bupd_iter_frame_l. apply bupd_iter_mono.
   iIntros "[Hback H]".
-  iDestruct "H" as (e2' l2' t2') "(% & (Hw&HE&Hσ) & _)"; subst.
+  iDestruct "H" as (e2' t2') "(% & (Hw&HE&Hσ) & _)"; subst.
   rewrite fupd_eq.
   iMod ("Hback" with "Hσ [$Hw $HE]") as "> (_ & _ & $)"; auto.
 Qed.
 End adequacy.
 
-Theorem wp_adequacy Σ Λ `{invPreG Σ} e l σ φ :
+Theorem wp_adequacy Σ Λ `{invPreG Σ} e σ φ :
   (∀ `{Hinv : invG Σ},
-     True ={⊤}=∗ ∃ (stateI : state Λ → iProp Σ) (localI : local_state Λ → iProp Σ),
-       let _ : irisG Λ Σ := IrisG _ _ _ Hinv stateI localI in
+     True ={⊤}=∗ ∃ stateI : state Λ → iProp Σ,
+       let _ : irisG Λ Σ := IrisG _ _ Hinv stateI in
        stateI σ ∗ WP e {{ v, ⌜φ v⌝ }}) →
-  adequate e l σ φ.
+  adequate e σ φ.
 Proof.
   intros Hwp; split.
-  - intros t2 l2 σ2 v2 [n ?]%rtc_nsteps.
+  - intros l2 t2 σ2 v2 [n ?]%rtc_nsteps.
     eapply (soundness (M:=iResUR Σ) _ (S (S (S n)))); iIntros "".
     rewrite Nat_iter_S. iMod wsat_alloc as (Hinv) "[Hw HE]".
     rewrite fupd_eq in Hwp; iMod (Hwp with "[$Hw $HE]") as ">(Hw & HE & Hwp)".
-    iDestruct "Hwp" as (Istate Ilocal) "[HI Hwp]".
-    iModIntro. iNext. iApply (@wptp_result _ _ (IrisG _ _ _ Hinv Istate Ilocal)); eauto.
+    iDestruct "Hwp" as (Istate) "[HI Hwp]".
+    iModIntro. iNext. iApply (@wptp_result _ _ (IrisG _ _ Hinv Istate)); eauto.
     iFrame. by iApply big_sepL_nil.
-  - intros t2 l2 σ2 e2 [n ?]%rtc_nsteps ?.
+  - intros l2 t2 σ2 e2 [n ?]%rtc_nsteps ?.
     eapply (soundness (M:=iResUR Σ) _ (S (S (S n)))); iIntros "".
     rewrite Nat_iter_S. iMod wsat_alloc as (Hinv) "[Hw HE]".
     rewrite fupd_eq in Hwp; iMod (Hwp with "[$Hw $HE]") as ">(Hw & HE & Hwp)".
-    iDestruct "Hwp" as (Istate Ilocal) "[HI Hwp]".
-    iModIntro. iNext. iApply (@wptp_safe _ _ (IrisG _ _ _ Hinv Istate Ilocal)); eauto.
+    iDestruct "Hwp" as (Istate) "[HI Hwp]".
+    iModIntro. iNext. iApply (@wptp_safe _ _ (IrisG _ _ Hinv Istate) _ _ (e2, l2)); eauto.
     iFrame. by iApply big_sepL_nil.
 Qed.
 
-Theorem wp_invariance Σ Λ `{invPreG Σ} e l σ1 t2 σ2 φ Φ :
+Theorem wp_invariance Σ Λ `{invPreG Σ} e σ1 t2 σ2 φ Φ :
   (∀ `{Hinv : invG Σ},
-     True ={⊤}=∗ ∃ (stateI : state Λ → iProp Σ) (localI : local_state Λ → iProp Σ),
-       let _ : irisG Λ Σ := IrisG _ _ _ Hinv stateI localI in
+     True ={⊤}=∗ ∃ stateI : state Λ → iProp Σ,
+       let _ : irisG Λ Σ := IrisG _ _ Hinv stateI in
        stateI σ1 ∗ WP e {{ Φ }} ∗ (stateI σ2 ={⊤,∅}=∗ ⌜φ⌝)) →
-  rtc step ([(e, l)], σ1) (t2, σ2) →
+  rtc step ([e], σ1) (t2, σ2) →
   φ.
 Proof.
   intros Hwp [n ?]%rtc_nsteps.
   eapply (soundness (M:=iResUR Σ) _ (S (S (S n)))); iIntros "".
   rewrite Nat_iter_S. iMod wsat_alloc as (Hinv) "[Hw HE]".
   rewrite {1}fupd_eq in Hwp; iMod (Hwp with "[$Hw $HE]") as ">(Hw & HE & Hwp)".
-  iDestruct "Hwp" as (Istate Ilocal) "(HIstate & Hwp & Hclose)".
-  iModIntro. iNext. iApply (@wptp_invariance _ _ (IrisG _ _ _ Hinv Istate Ilocal)); eauto.
+  iDestruct "Hwp" as (Istate) "(HIstate & Hwp & Hclose)".
+  iModIntro. iNext. iApply (@wptp_invariance _ _ (IrisG _ _ Hinv Istate)); eauto.
   iFrame "Hw HE Hwp HIstate Hclose". by iApply big_sepL_nil.
 Qed.
