theories/program_logic/weakestpre.v
@@ -5,24 +5,24 @@ From iris.proofmode Require Import tactics classes.
 Set Default Proof Using "Type".
 Import uPred.
 
-Class irisG' (Λlocal Λstate : Type) (Σ : gFunctors) := IrisG {
+Class irisG' (Λstate : Type) (Σ : gFunctors) := IrisG {
   iris_invG :> invG Σ;
   state_interp : Λstate → iProp Σ;
-  local_interp : Λlocal → iProp Σ;
 }.
-Notation irisG Λ Σ := (irisG' (local_state Λ) (state Λ) Σ).
+
+Notation irisG Λ Σ := (irisG' (state Λ) Σ).
 
 Definition wp_pre `{irisG Λ Σ}
-    (wp : coPset -c> expr Λ -c> (val Λ -c> iProp Σ) -c> iProp Σ) :
-    coPset -c> expr Λ -c> (val Λ -c> iProp Σ) -c> iProp Σ := λ E e1 Φ, (
+    (wp : coPset -c> (expr Λ * local_state Λ) -c> (val Λ -c> iProp Σ) -c> iProp Σ) :
+    coPset -c> (expr Λ * local_state Λ) -c> (val Λ -c> iProp Σ) -c> iProp Σ := λ E e1 Φ, (
   (* value case *)
-  (∃ v, ⌜to_val e1 = Some v⌝ ∧ |={E}=> Φ v) ∨
+  (∃ v, ⌜to_val (e1.1) = Some v⌝ ∧ |={E}=> Φ v) ∨
   (* step case *)
-  (⌜to_val e1 = None⌝ ∧ ∀ l1 σ1,
-     state_interp σ1 ∗ local_interp l1 ={E,∅}=∗ ⌜reducible e1 l1 σ1⌝ ∗
-     ▷ ∀ e2 l2 σ2 efs, ⌜prim_step e1 l1 σ1 e2 l2 σ2 efs⌝ ={∅,E}=∗
-       state_interp σ2 ∗ local_interp l2 ∗ wp E e2 Φ ∗
-       [∗ list] ef ∈ efs, local_interp (init_local Λ) -∗ wp ⊤ ef (λ _, True)))%I.
+  (⌜to_val (e1.1) = None⌝ ∧ ∀ σ1,
+     state_interp σ1 ={E,∅}=∗ ⌜reducible (e1.1) (e1.2) σ1⌝ ∗
+     ▷ ∀ e2 σ2 efs, ⌜prim_step (e1.1) (e1.2) σ1 (e2.1) (e2.2) σ2 efs⌝ ={∅,E}=∗
+       state_interp σ2 ∗ wp E e2 Φ ∗
+       [∗ list] ef ∈ efs, wp ⊤ (ef, init_local Λ) (λ _, True)))%I.
 
 Local Instance wp_pre_contractive `{irisG Λ Σ} : Contractive wp_pre.
 Proof.
@@ -31,7 +31,7 @@ Proof.
 Qed.
 
 Definition wp_def `{irisG Λ Σ} :
-  coPset → expr Λ → (val Λ → iProp Σ) → iProp Σ := fixpoint wp_pre.
+  coPset → (expr Λ * local_state Λ) → (val Λ → iProp Σ) → iProp Σ := fixpoint wp_pre.
 Definition wp_aux : { x | x = @wp_def }. by eexists. Qed.
 Definition wp := proj1_sig wp_aux.
 Definition wp_eq : @wp = @wp_def := proj2_sig wp_aux.
@@ -97,7 +97,7 @@ Context `{irisG Λ Σ}.
 Implicit Types P : iProp Σ.
 Implicit Types Φ : val Λ → iProp Σ.
 Implicit Types v : val Λ.
-Implicit Types e : expr Λ.
+Implicit Types e : (expr Λ * local_state Λ).
 
 (* Weakest pre *)
 Lemma wp_unfold E e Φ : WP e @ E {{ Φ }} ⊣⊢ wp_pre wp E e Φ.
@@ -111,7 +111,7 @@ Proof.
   (* FIXME: figure out a way to properly automate this proof *)
   (* FIXME: reflexivity, as being called many times by f_equiv and f_contractive
   is very slow here *)
-  do 23 (f_contractive || f_equiv). apply IH; first lia.
+  do 18 (f_contractive || f_equiv). apply IH; first lia.
   intros v. eapply dist_le; eauto with omega.
 Qed.
 Global Instance wp_proper E e :
@@ -120,12 +120,13 @@ Proof.
   by intros Φ Φ' ?; apply equiv_dist=>n; apply wp_ne=>v; apply equiv_dist.
 Qed.
 
-Lemma wp_value' E Φ v : Φ v ⊢ WP of_val v @ E {{ Φ }}.
+Lemma wp_value' E Φ v s : Φ v ⊢ WP (of_val v, s) @ E {{ Φ }}.
 Proof.
   iIntros "HΦ". rewrite wp_unfold /wp_pre.
   iLeft; iExists v; rewrite to_of_val; auto.
 Qed.
-Lemma wp_value_inv E Φ v : WP of_val v @ E {{ Φ }} ={E}=∗ Φ v.
+
+Lemma wp_value_inv E Φ v s : WP (of_val v, s) @ E {{ Φ }} ={E}=∗ Φ v.
 Proof.
   rewrite wp_unfold /wp_pre to_of_val. iIntros "[H|[% _]]"; [|done].
   by iDestruct "H" as (v') "[% ?]"; simplify_eq.
@@ -138,20 +139,20 @@ Proof.
   iDestruct "H" as "[Hv|[% H]]"; [iLeft|iRight].
   { iDestruct "Hv" as (v) "[% Hv]". iExists v; iSplit; first done.
     iApply ("HΦ" with ">[-]"). by iApply (fupd_mask_mono E1 _). }
-  iSplit; [done|]; iIntros (l1 σ1) "Hσ".
+  iSplit; [done|]; iIntros (σ1) "Hσ".
   iMod (fupd_intro_mask' E2 E1) as "Hclose"; first done.
-  iMod ("H" $! l1 σ1 with "Hσ") as "[$ H]".
-  iModIntro. iNext. iIntros (e2 l2 σ2 efs Hstep).
-  iMod ("H" $! _ _ _ efs with "[#]") as "($ & $ & H & $)"; auto.
+  iMod ("H" $! σ1 with "Hσ") as "[$ H]".
+  iModIntro. iNext. iIntros (e2 σ2 efs Hstep).
+  iMod ("H" $! _ _ efs with "[#]") as "($ & H & $)"; auto.
   iMod "Hclose" as "_". by iApply ("IH" with "HΦ").
 Qed.
 
 Lemma fupd_wp E e Φ : (|={E}=> WP e @ E {{ Φ }}) ⊢ WP e @ E {{ Φ }}.
 Proof.
-  rewrite wp_unfold /wp_pre. iIntros "H". destruct (to_val e) as [v|] eqn:?.
+  rewrite wp_unfold /wp_pre. iIntros "H". destruct (to_val (e.1)) as [v|] eqn:?.
   { iLeft. iExists v; iSplit; first done.
     by iMod "H" as "[H|[% ?]]"; [iDestruct "H" as (v') "[% ?]"|]; simplify_eq. }
-  iRight; iSplit; [done|]; iIntros (l1 σ1) "Hσ1".
+  iRight; iSplit; [done|]; iIntros (σ1) "Hσ1".
   iMod "H" as "[H|[% H]]"; last by iApply "H".
   iDestruct "H" as (v') "[% ?]"; simplify_eq.
 Qed.
@@ -159,37 +160,39 @@ Lemma wp_fupd E e Φ : WP e @ E {{ v, |={E}=> Φ v }} ⊢ WP e @ E {{ Φ }}.
 Proof. iIntros "H". iApply (wp_strong_mono E); try iFrame; auto. Qed.
 
 Lemma wp_atomic E1 E2 e Φ :
-  atomic e →
+  atomic (e.1) →
   (|={E1,E2}=> WP e @ E2 {{ v, |={E2,E1}=> Φ v }}) ⊢ WP e @ E1 {{ Φ }}.
 Proof.
-  iIntros (Hatomic) "H". destruct (to_val e) as [v|] eqn:He.
+  iIntros (Hatomic) "H". destruct e.
+  destruct (to_val e) as [v|] eqn:He.
   { apply of_to_val in He as <-. iApply wp_fupd. iApply wp_value'.
     iMod "H". by iMod (wp_value_inv with "H"). }
   setoid_rewrite wp_unfold; rewrite /wp_pre. iRight; iSplit; auto.
-  iIntros (l1 σ1) "Hσ". iMod "H" as "[H|[_ H]]".
-  { iDestruct "H" as (v') "[% ?]"; simplify_eq. }
-  iMod ("H" $! _ _ with "Hσ") as "[$ H]".
-  iModIntro. iNext. iIntros (e2 l2 σ2 efs Hstep).
-  iMod ("H" with "* []") as "(Hphy & Hl & H & $)"; first done.
+  iIntros (σ1) "Hσ". iMod "H" as "[H|[_ H]]".
+  { iDestruct "H" as (v') "[% ?]"; simpl in *. simplify_eq. }
+  iMod ("H" $! _ with "Hσ") as "[$ H]".
+  iModIntro. iNext. iIntros (e2 σ2 efs Hstep).
+  iMod ("H" with "* []") as "(Hphy & H & $)"; first done.
   rewrite wp_unfold /wp_pre. iDestruct "H" as "[H|H]".
   - iDestruct "H" as (v) "[% >>?]". iModIntro. iFrame.
-    rewrite -(of_to_val e2 v) //. by iApply wp_value'.
+    destruct e2. simpl in *.
+    rewrite -(of_to_val e0 v) //. by iApply wp_value'.
   - iDestruct "H" as "[_ H]".
-    iMod ("H" with "* [Hphy Hl]") as "[H _]"; first iFrame.
+    iMod ("H" with "* Hphy") as "[H _]"; first iFrame.
     iDestruct "H" as %(? & ? & ? & ? & ?). exfalso.
     by eapply (Hatomic _ _ _ _ _ _ Hstep).
 Qed.
 
 Lemma wp_fupd_step E1 E2 e P Φ :
-  to_val e = None → E2 ⊆ E1 →
+  to_val (e.1) = None → E2 ⊆ E1 →
   (|={E1,E2}▷=> P) -∗ WP e @ E2 {{ v, P ={E1}=∗ Φ v }} -∗ WP e @ E1 {{ Φ }}.
 Proof.
   rewrite !wp_unfold /wp_pre. iIntros (??) "HR [Hv|[_ H]]".
   { iDestruct "Hv" as (v) "[% Hv]"; simplify_eq. }
-  iRight; iSplit; [done|]. iIntros (l1 σ1) "[Hσ Hl]".
-  iMod "HR". iMod ("H" $! _ _ with "[Hσ Hl]") as "[$ H]"; first iFrame.
-  iModIntro; iNext; iIntros (e2 l2 σ2 efs Hstep).
-  iMod ("H" $! e2 l2 σ2 efs with "[%]") as "($ & $ & H & $)"; auto=>//.
+  iRight; iSplit; [done|]. iIntros (σ1) "Hσ".
+  iMod "HR". iMod ("H" $! _ with "Hσ") as "[$ H]"; first iFrame.
+  iModIntro; iNext; iIntros (e2 σ2 efs Hstep).
+  iMod ("H" $! e2 σ2 efs with "[%]") as "($ & H & $)"; auto=>//.
   iMod "HR". iModIntro. iApply (wp_strong_mono E2); first done.
   iSplitR "H"; last iExact "H". iIntros (v) "H". by iApply "H".
 Qed.
@@ -206,12 +209,12 @@ Global Instance wp_mono' E e :
   Proper (pointwise_relation _ (⊢) ==> (⊢)) (@wp Λ Σ _ E e).
 Proof. by intros Φ Φ' ?; apply wp_mono. Qed.
 
-Lemma wp_value E Φ e v : to_val e = Some v → Φ v ⊢ WP e @ E {{ Φ }}.
-Proof. intros; rewrite -(of_to_val e v) //; by apply wp_value'. Qed.
-Lemma wp_value_fupd' E Φ v : (|={E}=> Φ v) ⊢ WP of_val v @ E {{ Φ }}.
+Lemma wp_value E Φ e v : to_val (e.1) = Some v → Φ v ⊢ WP e @ E {{ Φ }}.
+Proof. intros. destruct e. rewrite -(of_to_val e v) //; by apply wp_value'. Qed.
+Lemma wp_value_fupd' E Φ v s : (|={E}=> Φ v) ⊢ WP (of_val v, s) @ E {{ Φ }}.
 Proof. intros. by rewrite -wp_fupd -wp_value'. Qed.
 Lemma wp_value_fupd E Φ e v :
-  to_val e = Some v → (|={E}=> Φ v) ⊢ WP e @ E {{ Φ }}.
+  to_val (e.1) = Some v → (|={E}=> Φ v) ⊢ WP e @ E {{ Φ }}.
 Proof. intros. rewrite -wp_fupd -wp_value //. Qed.
 
 Lemma wp_frame_l E e Φ R : R ∗ WP e @ E {{ Φ }} ⊢ WP e @ E {{ v, R ∗ Φ v }}.
@@ -220,24 +223,24 @@ Lemma wp_frame_r E e Φ R : WP e @ E {{ Φ }} ∗ R ⊢ WP e @ E {{ v, Φ v ∗ 
 Proof. iIntros "[??]". iApply (wp_strong_mono E E _ Φ); try iFrame; eauto. Qed.
 
 Lemma wp_frame_step_l E1 E2 e Φ R :
-  to_val e = None → E2 ⊆ E1 →
+  to_val (e.1) = None → E2 ⊆ E1 →
   (|={E1,E2}▷=> R) ∗ WP e @ E2 {{ Φ }} ⊢ WP e @ E1 {{ v, R ∗ Φ v }}.
 Proof.
   iIntros (??) "[Hu Hwp]". iApply (wp_fupd_step with "Hu"); try done.
   iApply (wp_mono with "Hwp"). by iIntros (?) "$$".
 Qed.
 Lemma wp_frame_step_r E1 E2 e Φ R :
-  to_val e = None → E2 ⊆ E1 →
+  to_val (e.1) = None → E2 ⊆ E1 →
   WP e @ E2 {{ Φ }} ∗ (|={E1,E2}▷=> R) ⊢ WP e @ E1 {{ v, Φ v ∗ R }}.
 Proof.
   rewrite [(WP _ @ _ {{ _ }} ∗ _)%I]comm; setoid_rewrite (comm _ _ R).
   apply wp_frame_step_l.
 Qed.
 Lemma wp_frame_step_l' E e Φ R :
-  to_val e = None → ▷ R ∗ WP e @ E {{ Φ }} ⊢ WP e @ E {{ v, R ∗ Φ v }}.
+  to_val (e.1) = None → ▷ R ∗ WP e @ E {{ Φ }} ⊢ WP e @ E {{ v, R ∗ Φ v }}.
 Proof. iIntros (?) "[??]". iApply (wp_frame_step_l E E); try iFrame; eauto. Qed.
 Lemma wp_frame_step_r' E e Φ R :
-  to_val e = None → WP e @ E {{ Φ }} ∗ ▷ R ⊢ WP e @ E {{ v, Φ v ∗ R }}.
+  to_val (e.1) = None → WP e @ E {{ Φ }} ∗ ▷ R ⊢ WP e @ E {{ v, Φ v ∗ R }}.
 Proof. iIntros (?) "[??]". iApply (wp_frame_step_r E E); try iFrame; eauto. Qed.
 
 Lemma wp_wand E e Φ Ψ :
@@ -277,7 +280,7 @@ Section proofmode_classes.
 
   (* lower precedence, if possible, it should always pick elim_upd_fupd_wp *)
   Global Instance elim_modal_fupd_wp_atomic E1 E2 e P Φ :
-    atomic e →
+    atomic (e.1) →
     ElimModal (|={E1,E2}=> P) P
             (WP e @ E1 {{ Φ }}) (WP e @ E2 {{ v, |={E2,E1}=> Φ v }})%I | 100.
   Proof. intros. by rewrite /ElimModal fupd_frame_r wand_elim_r wp_atomic. Qed.
