theories/tests/higher_order.v
@@ -1,23 +1,21 @@
-Require Import iris_c.clang.logic.
+From iris_c.clang Require Import logic notations.
 
 Section example.
   Context `{clangG Σ}.
 
   Definition abs_spec g E (P Q: iProp Σ) :=
     (∃ gbody, text_interp g (Function Tvoid [] gbody) ∗
-              (∀ Φ, P -∗ (Q -∗ Φ Vvoid) -∗ WP gbody @ E {{ Φ }}))%I.
+              (∀ Φ k ks, P -∗ (Q -∗ WP (fill_ectxs void k, ks) {{ Φ }}) -∗ WP (gbody, k::ks) @ E {{ Φ }}))%I.
 
-  Lemma higher_order_spec ks E g Φ P Q:
-    abs_spec g E P Q ∗ P ∗
-    own_stack ks ∗ (own_stack ([]::ks) -∗ Q -∗ Φ Vvoid)
-    ⊢ WP Ecall Tvoid g [] @ E {{ Φ }}.
+  Lemma higher_order_spec k ks E g Φ P Q:
+    abs_spec g E P Q ∗ P ∗ (Q -∗ WP (fill_ectxs void k, ks) {{ Φ }})
+    ⊢ WP (fill_ectxs (Ecall Tvoid g []) k, ks) @ E {{ Φ }}.
   Proof.
-    iIntros "(Hg & HP & Hs & HΦ)".
+    iIntros "(Hg & HP & HΦ)".
     iDestruct "Hg" as (e) "[Ht He]".
-    iApply (wp_call [] []); last iFrame; first done.
-    iNext. iIntros "Hs'".
-    iApply ("He" with "HP").
-    by iApply "HΦ".
+    iApply (wp_call _ []); last iFrame; first done.
+    iNext. iApply ("He" with "HP").
+    iApply "HΦ".
   Qed.
 
 End example.
