theories/clang/adequacy.v
@@ -1,14 +1,13 @@
-From iris_os.clang Require Export logic.
+From iris_c.clang Require Export logic.
 From iris_c.program_logic Require Import weakestpre adequacy.
 
 Class clangPreG Σ := ClangPreG {
   clang_preG_iris :> invPreG Σ;
   clang_preG_clang :> gen_heapPreG addr byteval Σ;
   clangG_preG_textG :> inG Σ textG;
-  clangG_preG_stackG :> inG Σ stackG;
 }.
 
-Definition clangΣ : gFunctors := #[invΣ; gen_heapΣ addr byteval; GFunctor textG; GFunctor stackG].
+Definition clangΣ : gFunctors := #[invΣ; gen_heapΣ addr byteval; GFunctor textG].
 Instance subG_clangPreG {Σ} : subG clangΣ Σ → clangPreG Σ.
 Proof. solve_inG. Qed.
 
@@ -21,10 +20,8 @@ Proof.
   { apply: auth_auth_valid. exact: to_gen_heap_valid. }
   iMod (own_alloc (● to_gen_text (s_text σ))) as (γ') "Ht".
   { apply: auth_auth_valid. intros l. rewrite lookup_fmap. by case (s_text σ !! l).  }
-  iMod (own_alloc (to_gen_stack (s_stack σ))) as (γ'') "Hs"; first split=>//.
   iModIntro. iExists (fun σ => own γ (● to_gen_heap (s_heap σ)) ∗
-                               own γ' (● to_gen_text (s_text σ)) ∗
-                               own γ'' (to_gen_stack (s_stack σ)))%I.
+                               own γ' (● to_gen_text (s_text σ)))%I.
   set (Hheap := GenHeapG addr byteval Σ _ _ _ γ).
-  iFrame. iApply (Hwp (ClangG _ _ _ _ γ' _ γ'')).
+  iFrame. iApply (Hwp (ClangG _ _ _ _ γ')).
 Qed.
