theories/clang/lib/page_table.v
@@ -16,21 +16,22 @@ Structure page_table Σ `{!clangG Σ} :=  {
   (* -- predicates -- *)
   is_page_table: gmap int32 addr → iProp Σ;
   (* -- operation specs -- *)
-  insert_pt_spec i l m Φ:
+  insert_pt_spec i l m Φ ks:
     is_page_table m ∗ (is_page_table (<[ i := l ]> m) -∗ Φ Vvoid)
-    ⊢ WP (Ecall Tvoid insert_pt [Evalue (Vint32 i); Evalue (Vptr l)]) {{ Φ }};
-  delete_pt_spec i m Φ:
+    ⊢ WP (Ecall Tvoid insert_pt [Evalue (Vint32 i); Evalue (Vptr l)], ks) {{ Φ }};
+  delete_pt_spec i m Φ ks:
     is_page_table m ∗ (is_page_table (delete i m) -∗ Φ Vvoid)
-    ⊢ WP (Ecall Tvoid delete_pt [Evalue (Vint32 i)]) {{ Φ }};
-  lookup_pt_spec i m Φ:
+    ⊢ WP (Ecall Tvoid delete_pt [Evalue (Vint32 i)], ks) {{ Φ }};
+  lookup_pt_spec i m Φ ks:
     is_page_table m ∗ (is_page_table m -∗ Φ (option_addr_to_val (m !! i)))
-    ⊢ WP (Ecall (Tptr Tvoid) lookup_pt [Evalue (Vint32 i)]) {{ Φ }}
+    ⊢ WP (Ecall (Tptr Tvoid) lookup_pt [Evalue (Vint32 i)], ks) {{ Φ }}
 }.
 
 Arguments insert_pt {_ _} _.
 Arguments delete_pt {_ _} _.
 Arguments lookup_pt {_ _} _.
-Arguments insert_pt_spec {_ _} _ _ _ _ _.
-Arguments delete_pt_spec {_ _} _ _ _ _.
-Arguments lookup_pt_spec {_ _} _ _ _ _.
+Arguments insert_pt_spec {_ _} _ _ _ _ _ _.
+Arguments delete_pt_spec {_ _} _ _ _ _ _.
+Arguments lookup_pt_spec {_ _} _ _ _ _ _.
 Arguments is_page_table {_ _} _ _.
+
