theories/clang/logic.v
@@ -19,8 +19,6 @@ Class clangG Σ := ClangG {
   clangG_heapG :> gen_heapG addr byteval Σ;
   clangG_textG :> inG Σ textG;
   clangG_textG_name : gname;
-  clangG_stackG :> @pairG stack Σ;
-  clangG_stackG_name : gname
 }.
 
 Section wp.
@@ -33,9 +31,6 @@ Section wp.
     text_interp f x ⊢ text_interp f x ∗ text_interp f x.
   Admitted.
   
-  Definition own_stack :=
-    @own_pair stack Σ clangG_stackG clangG_stackG_name.
-
   Definition to_gen_text (t: text) :=
     fmap (λ v, to_agree (v : leibnizC function)) t.
 
@@ -60,7 +55,6 @@ End wp.
 Instance heapG_irisG `{clangG Σ}: irisG clang_lang Σ := {
   iris_invG := clangG_invG;
   state_interp := clang_state_interp;
-  local_interp := own_stack
 }.
 
 Global Opaque iris_invG.
@@ -88,106 +82,84 @@ Section rules.
   Global Instance timeless_mapstoval p q v t : TimelessP (p ↦{q} v @ t)%I.
   Proof. rewrite /mapstoval. apply _. Qed.
 
-  Lemma wp_bind' kes E e Φ :
+  Lemma wp_bind' kes E e s Φ :
     ⌜ is_jmp e = false ⌝ ∗
-    WP e @ E {{ v, WP (fill_ectxs (Evalue v) kes) @ E {{ Φ }} }}
-    ⊢ WP (fill_ectxs e kes) @ E {{ Φ }}.
+    WP (e, s) @ E {{ v, WP (fill_ectxs (Evalue v) kes, s) @ E {{ Φ }} }}
+    ⊢ WP (fill_ectxs e kes, s) @ E {{ Φ }}.
   Proof.
-    iIntros "H". iLöb as "IH" forall (E e Φ). rewrite wp_unfold /wp_pre.
+    iIntros "H". iLöb as "IH" forall (E e s Φ). rewrite wp_unfold /wp_pre.
     iDestruct "H" as "[% [Hv|[% H]]]".
-    { iDestruct "Hv" as (v) "[Hev Hv]";
+    { simpl. iDestruct "Hv" as (v) "[Hev Hv]";
         iDestruct "Hev" as % <-%of_to_val.
         by iApply fupd_wp. }
     rewrite wp_unfold /wp_pre.
     iRight; iSplit; eauto using fill_ectxs_not_val.
-    iIntros (l1 σ1) "Hσ". iMod ("H" $! _ _ with "Hσ") as "[% H]".
+    iIntros (σ1) "Hσ". iMod ("H" $! _ with "Hσ") as "[% H]".
     iModIntro; iSplit.
     { iPureIntro. unfold reducible in *.
       destruct H2 as (cur'&?&?σ'&efs&?). eexists _, _, _, _.
       apply CSbind=>//. }
-    iNext. iIntros (e2 l2 σ2 efs Hstep).
-    edestruct (fill_step_inv e σ1 e2 σ2 l1 l2 kes) as (e2'&->&?&?); auto; subst=>//.
-    iMod ("H" $! _ _ _ _ with "[%]") as "($ & $ & H & Hefs)"; eauto.
+    iNext. iIntros (e2 σ2 efs Hstep). simpl in *.
+    destruct e2 as [e2 l2].
+    edestruct (fill_step_inv e σ1 e2 σ2 s l2 kes) as (e2'&->&?&?); auto; subst=>//.
+    iMod ("H" $! (e2', l2) _ _ with "[%]") as "($ & H & Hefs)"; eauto.
     iFrame "Hefs". iApply "IH". iSplit=>//.
     iPureIntro. eapply cstep_preserves_not_jmp=>//.
   Qed.
 
-  Lemma wp_bind kes E e Φ :
+  Lemma wp_bind kes E e s Φ :
     is_jmp e = false →
-    WP e @ E {{ v, WP (fill_ectxs (Evalue v) kes) @ E {{ Φ }} }}
-    ⊢ WP (fill_ectxs e kes) @ E {{ Φ }}.
+    WP (e, s) @ E {{ v, WP (fill_ectxs (Evalue v) kes, s) @ E {{ Φ }} }}
+    ⊢ WP (fill_ectxs e kes, s) @ E {{ Φ }}.
   Proof. iIntros (?) "?". iApply wp_bind'. iSplit; done. Qed.
 
   Definition reducible := @reducible clang_lang.
 
   Lemma wp_lift_step E Φ e1 :
-    to_val e1 = None →
-    (∀ l1 σ1, state_interp σ1 ∗ local_interp l1 ={E,∅}=∗
-      ⌜ reducible e1 l1 σ1⌝ ∗
-      ▷ ∀ e2 l2 σ2 efs, ⌜cstep e1 l1 σ1 e2 l2 σ2 efs⌝ ={∅,E}=∗
-        state_interp σ2 ∗ local_interp l2 ∗ WP e2 @ E {{ Φ }} ∗ [∗ list] ef ∈ efs, own_stack [] -∗ WP ef {{ _, True }})
+    to_val (e1.1) = None →
+    (∀ σ1, state_interp σ1 ={E,∅}=∗
+      ⌜ reducible (e1.1) (e1.2) σ1⌝ ∗
+      ▷ ∀ e2 σ2 efs, ⌜cstep (e1.1) (e1.2) σ1 (e2.1) (e2.2) σ2 efs⌝ ={∅,E}=∗
+        state_interp σ2 ∗ WP e2 @ E {{ Φ }} ∗ [∗ list] ef ∈ efs, WP (ef, []) {{ _, True }})
     ⊢ WP e1 @ E {{ Φ }}.
   Proof. iIntros (?) "H". rewrite wp_unfold /wp_pre; auto. Qed.
 
-  Lemma wp_lift_pure_step E Φ e1 :
-    (∀ l1 σ1, reducible e1 l1 σ1) →
+  Lemma wp_lift_pure_step E Φ e1 l1 :
+    (∀ σ1, reducible e1 l1 σ1) →
     (∀ σ1 σ2 cur2 l1 l2 efs, cstep e1 l1 σ1 cur2 l2 σ2 efs → σ1 = σ2 ∧ l1 = l2) →
-    (▷ ∀ cur2 l1 l2 σ1 σ2 efs, ⌜ cstep e1 l1 σ1 cur2 l2 σ2 efs ⌝ →
-                WP cur2 @ E {{ Φ }} ∗ [∗ list] ef ∈ efs, own_stack [] -∗ WP ef {{ _, True }})
-      ⊢ WP e1 @ E {{ Φ }}.
+    (▷ ∀ e2 l2 σ1 σ2 efs, ⌜ cstep e1 l1 σ1 e2 l2 σ2 efs ⌝ →
+                          WP (e2, l2) @ E {{ Φ }} ∗ [∗ list] ef ∈ efs, WP (ef, []) {{ _, True }})
+      ⊢ WP (e1, l1) @ E {{ Φ }}.
   Proof.
     iIntros (Hsafe Hs) "H".
     iApply wp_lift_step.
-    { eapply (@reducible_not_val clang_lang), (Hsafe inhabitant inhabitant). }
-    iIntros (l1 σ1) "[? ?]". iMod (fupd_intro_mask' E ∅) as "Hclose"; first set_solver.
-    iModIntro. iSplit; [done|]; iNext; iIntros (e2 l2 σ2 ? Hsp).
+    { eapply (@reducible_not_val clang_lang), (Hsafe inhabitant). }
+    iIntros (σ1) "?". iMod (fupd_intro_mask' E ∅) as "Hclose"; first set_solver.
+    iModIntro. iSplit; [done|]; iNext; iIntros (e2 σ2 ? Hsp).
     iMod "Hclose"; iModIntro.
     destruct (Hs _ _ _ _ _ _ Hsp) as [? ?]. subst. iFrame.
-    by iApply "H".
-  Qed.
-  
-  Lemma stack_pop k k' ks ks':
-    own_stack (k::ks) ∗ own_stack (k'::ks') ==∗
-    own_stack (ks) ∗ own_stack (ks') ∗ ⌜ k = k' ∧ ks = ks' ⌝.
-  Proof.
-    iIntros "[Hs Hs']".
-    iMod (own_pair_update with "[-]") as "[? [? %]]"; first iFrame.
-    inversion H0. by iFrame.
-  Qed.
-
-  Lemma stack_push k ks ks':
-    own_stack (ks) ∗ own_stack (ks') ==∗
-    own_stack (k::ks) ∗ own_stack (k::ks') ∗ ⌜ ks = ks' ⌝.
-  Proof.
-    iIntros "[Hs Hs']".
-    iMod (own_pair_update with "[-]") as "[? [? %]]"; first iFrame.
-    inversion H0. by iFrame.
+    simpl in *. destruct e2. by iApply "H".
   Qed.
 
   Lemma wp_ret k k' ks v E Φ:
-    own_stack (k'::ks) ∗
-    (own_stack ks -∗ WP fill_ectxs (Evalue v) k' @ E {{ Φ }})
-    ⊢ WP fill_ectxs (Erete (Evalue v)) k @ E {{ Φ }}.
+    WP (fill_ectxs (Evalue v) k', ks) @ E {{ Φ }}
+    ⊢ WP (fill_ectxs (Erete (Evalue v)) k, k'::ks) @ E {{ Φ }}.
   Proof.
-    iIntros "[Hs HΦ]".
+    iIntros "HΦ".
     iApply wp_lift_step; eauto; first by apply fill_ectxs_not_val.
-    iIntros (l σ) "[[Hσ HΓ] Hstk]".
+    iIntros (σ) "[Hσ HΓ]".
     iMod (fupd_intro_mask' _ ∅) as "Hclose"; first set_solver.
     iModIntro. iSplit.
-    { iDestruct (own_pair_agree with "[Hstk Hs]") as "%"; first iFrame.
-      subst. iPureIntro. destruct σ. eexists _, _, (State s_heap s_text), _.
+    { iPureIntro. destruct σ. simpl. eexists _, _, (State s_heap s_text), _.
       apply CSjstep. simpl in *. subst. constructor.
       apply cont_uninj. auto. }
-    iNext. iIntros (e2 l2 σ2 efs Hcs).
+    iNext. iIntros (e2 σ2 efs Hcs).
     inversion_cstep_as Hes Hjs; subst.
-    { by apply fill_estep_false in Hes. }
-    inversion_jstep_as Heq; subst.
-    apply cont_inj in Heq=>//; auto;
-    destruct Heq as [Heq ?]; inversion Heq; subst.
-    iMod (stack_pop with "[Hstk Hs]") as "(Hstk & Hs & %)"; first iFrame.
-    destruct H1; subst. iFrame. iMod "Hclose" as "_".
-    iModIntro. iSplitL; first by iApply "HΦ".
-      by rewrite big_sepL_nil.
+    { destruct e2. simpl in *. by apply fill_estep_false in Hes. }
+    destruct e2. simpl in *. inversion_jstep_as Heq; subst.
+    - apply cont_inj in Heq=>//; auto;
+      destruct Heq as [Heq ?]; inversion Heq; subst.
+      iFrame. by rewrite big_sepL_nil.
     - fill_enf_neq.
   Qed.
 
@@ -200,8 +172,8 @@ Section rules.
     escape_false.
   Qed.
 
-  Lemma wp_skip E Φ v s:
-    ▷ WP s @ E {{ Φ }} ⊢ WP Eseq (Evalue v) s @ E {{ Φ }}.
+  Lemma wp_skip E Φ v s k:
+    ▷ WP (s, k) @ E {{ Φ }} ⊢ WP (Eseq (Evalue v) s, k) @ E {{ Φ }}.
   Proof.
     iIntros "Φ". iApply wp_lift_pure_step; eauto.
     - destruct σ1. eexists _, _, _, _. simpl. eauto.
@@ -214,7 +186,7 @@ Section rules.
         * unfold unfill in H2. rewrite H0 in H2.
           by simpl in *.
         * fill_enf_neq.
-    - iNext. iIntros (???????).
+    - iNext. iIntros (??????).
       inversion_cstep_as Hes Hjs; subst.
       + inversion Hes; subst.
         { iFrame. by rewrite big_sepL_nil. }
@@ -224,26 +196,26 @@ Section rules.
         * fill_enf_neq.
   Qed.
 
-  Lemma wp_seq E e1 e2 Φ:
+  Lemma wp_seq E e1 e2 l Φ:
     is_jmp e1 = false →
-    WP e1 @ E {{ v, WP Eseq (Evalue v) e2 @ E {{ Φ }} }} ⊢ WP Eseq e1 e2 @ E {{ Φ }}.
+    WP (e1, l) @ E {{ v, WP (Eseq (Evalue v) e2, l) @ E {{ Φ }} }} ⊢ WP (Eseq e1 e2, l) @ E {{ Φ }}.
   Proof. iIntros (?) "Hseq". iApply (wp_bind [EKseq e2])=>//. Qed.
 
-  Lemma wp_lift_atomic_step {E Φ} s1 :
+  Lemma wp_lift_atomic_step {E Φ} s1 l1 :
     to_val s1 = None →
-    (∀ l1 σ1, state_interp σ1 ∗ local_interp l1 ={E}=∗
+    (∀ l1 σ1, state_interp σ1 ={E}=∗
       ⌜reducible s1 l1 σ1⌝ ∗
       ▷ ∀ s2 l2 σ2 efs, ⌜cstep s1 l1 σ1 s2 l2 σ2 efs⌝ ={E}=∗
-        state_interp σ2 ∗ local_interp l2 ∗
-        default False (to_val s2) Φ  ∗ [∗ list] ef ∈ efs, own_stack [] -∗ WP ef {{ _, True }})
-    ⊢ WP s1 @ E {{ Φ }}.
+        state_interp σ2 ∗
+        default False (to_val s2) Φ  ∗ [∗ list] ef ∈ efs, WP (ef, []) {{ _, True }})
+    ⊢ WP (s1, l1) @ E {{ Φ }}.
   Proof.
-    iIntros (?) "H". iApply (wp_lift_step E _ s1)=>//; iIntros (l1 σ1) "[Hσ1 Hl1]".
-    iMod ("H" $! l1 σ1 with "[Hσ1 Hl1]") as "[$ H]"; first iFrame.
+    iIntros (?) "H". iApply (wp_lift_step E _ (s1, l1))=>//; iIntros (σ1) "Hσ1".
+    iMod ("H" $! l1 σ1 with "Hσ1") as "[$ H]"; first iFrame.
     iMod (fupd_intro_mask' E ∅) as "Hclose"; first set_solver.
-    iModIntro; iNext; iIntros (s2 l2 σ2 ? ?). iMod "Hclose" as "_".
-    iMod ("H" $! _ _ _ _ with "[#]") as "($ & $ & H & ?)"=>//. iFrame.
-    destruct (to_val s2) eqn:?; last by iExFalso.
+    iModIntro; iNext; iIntros (s2 σ2 ? ?). iMod "Hclose" as "_".
+    iMod ("H" $! _ _ _ _ with "[#]") as "($ & H & ?)"=>//. iFrame.
+    destruct (to_val (s2.1)) eqn:?; last by iExFalso.
     iApply wp_value=>//.
   Qed.
 
@@ -262,16 +234,16 @@ Section rules.
       by iFrame.
   Qed.
 
-  Lemma wp_assign {E l v v'} t t' Φ:
+  Lemma wp_assign {E l v v'} t t' ks Φ:
     typeof v' t' → assign_type_compatible t t' →
     ▷ l ↦ v @ t ∗ ▷ (l ↦ v' @ t -∗ Φ Vvoid)
-    ⊢ WP Eassign (Evalue (Vptr l)) (Evalue v') @ E {{ Φ }}.
+    ⊢ WP (Eassign (Evalue (Vptr l)) (Evalue v'), ks) @ E {{ Φ }}.
   Proof.
     iIntros (??) "[Hl HΦ]".
     iApply wp_lift_atomic_step=>//.
-    iIntros (l1 σ1) "[[Hσ HΓ] ?] !>".
+    iIntros (l1 σ1) "[Hσ HΓ] !>".
     rewrite /mapstoval. iSplit; first eauto.
-    { iPureIntro. destruct σ1. eexists _, _, _. simpl. eauto. }
+    { iPureIntro. destruct σ1. eexists _, _, _, _. simpl. eauto. }
     iNext; iIntros (v2 l2 σ2 efs Hstep).
     iDestruct "Hl" as "[% Hl]".
     iDestruct (gen_heap_update_bytes _ (encode_val v)
@@ -349,13 +321,13 @@ Section rules.
     l ↦{q} v @ t ⊢ ⌜ typeof v t ⌝.
   Proof. by iDestruct 1 as "[% ?]". Qed.
 
-  Lemma wp_load {E} Φ p v t q:
+  Lemma wp_load {E} ks Φ p v t q:
     ▷ p ↦{q} v @ t ∗ ▷ (p ↦{q} v @ t -∗ Φ v)
-    ⊢ WP Ederef_typed t (Evalue (Vptr p)) @ E {{ Φ }}.
+    ⊢ WP (Ederef_typed t (Evalue (Vptr p)), ks) @ E {{ Φ }}.
   Proof.
     iIntros "[Hl HΦ]".
     iApply wp_lift_atomic_step=>//.
-    iIntros (l1 σ1) "[[Hσ HΓ] Hs]".
+    iIntros (l1 σ1) "[Hσ HΓ]".
     unfold mapstoval.
     iDestruct "Hl" as "[>% >Hl]".
     iDestruct (mapsto_readbytes with "[Hσ Hl]") as "%"; first iFrame.
@@ -368,14 +340,14 @@ Section rules.
     iApply ("HΦ" with "[-]") ; first by iSplit=>//.
   Qed.
 
-  Lemma wp_cas_fail Φ E l t q v' v1 v2 :
+  Lemma wp_cas_fail Φ E ks l t q v' v1 v2 :
     v' ≠ v1 → typeof v1 t → typeof v2 t → (* too strong, should mimick wp_assign *)
     ▷ l ↦{q} v' @ t ∗ ▷ (l ↦{q} v' @ t -∗ Φ vfalse)
-    ⊢ WP ECAS t (Evalue (Vptr l)) (Evalue v1) (Evalue v2) @ E {{ Φ }}.
+    ⊢ WP (ECAS t (Evalue (Vptr l)) (Evalue v1) (Evalue v2), ks) @ E {{ Φ }}.
   Proof.
     iIntros (???) "[Hl HΦ]".
     iApply wp_lift_atomic_step=>//.
-    iIntros (l1 σ1) "[[Hσ HΓ] Hs]".
+    iIntros (l1 σ1) "[Hσ HΓ]".
     unfold mapstoval.
     iDestruct "Hl" as "[>% >Hl]".
     iDestruct (mapsto_readbytes with "[Hσ Hl]") as "%"; first iFrame.
@@ -393,14 +365,14 @@ Section rules.
     - absurd_jstep Hjs.
   Qed.
 
-  Lemma wp_cas_suc Φ E l t v v2 :
+  Lemma wp_cas_suc Φ E ks l t v v2 :
     typeof v t → typeof v2 t → (* too strong, should mimick wp_assign *)
     ▷ l ↦ v @ t ∗ ▷ (l ↦ v2 @ t -∗ Φ vtrue)
-    ⊢ WP ECAS t (Evalue (Vptr l)) (Evalue v) (Evalue v2) @ E {{ Φ }}.
+    ⊢ WP (ECAS t (Evalue (Vptr l)) (Evalue v) (Evalue v2), ks) @ E {{ Φ }}.
   Proof.
     iIntros (??) "[Hl HΦ]".
     iApply wp_lift_atomic_step=>//.
-    iIntros (l1 σ1) "[[Hσ HΓ] Hs]".
+    iIntros (l1 σ1) "[Hσ HΓ]".
     unfold mapstoval.
     iDestruct "Hl" as "[>% >Hl]".
     iDestruct (mapsto_readbytes with "[Hσ Hl]") as "%"; first iFrame.
@@ -424,38 +396,50 @@ Section rules.
     - absurd_jstep Hjs.
   Qed.
 
+Ltac atomic_step H :=
+  inversion H; subst;
+  [ match goal with
+    | [ HE: estep _ _ _ _ _ _ |- _ ] =>
+      inversion HE; subst;
+      [ idtac | exfalso; by escape_false ]
+    end
+  | match goal with
+    | [ HJ : jstep _ _ _ _ _ |- _ ] => absurd_jstep HJ
+    end
+  ].
+  
   Ltac wp_solve_pure :=
-    iApply wp_lift_pure_step; first eauto;
+    iApply wp_lift_pure_step;
     [ intros; solve_red |
       intros ???????Hcs; atomic_step Hcs=>// |
       iNext;
       let Hcs := fresh "Hcs" in
-      iIntros (???????Hcs);
+      iIntros (??????Hcs);
       atomic_step Hcs; iSplitL; last by rewrite big_sepL_nil ].
   
-  Lemma wp_op E op v1 v2 v' Φ:
+  Lemma wp_op E ks op v1 v2 v' Φ:
     evalbop op v1 v2 = Some v' →
-    Φ v' ⊢ WP Ebinop op (Evalue v1) (Evalue v2) @ E {{ Φ }}.
+    Φ v' ⊢ WP (Ebinop op (Evalue v1) (Evalue v2), ks) @ E {{ Φ }}.
   Proof.
     iIntros (?) "HΦ". wp_solve_pure.
     simplify_eq. subst. iApply wp_value=>//.
   Qed.
 
-  Lemma wp_while_true cond s Φ:
-    ▷ WP Eseq s (Ewhile cond cond s) {{ Φ }}
-    ⊢ WP Ewhile cond (Evalue vtrue) s {{ Φ }}.
+  Lemma wp_while_true cond s Φ ks:
+    ▷ WP (Eseq s (Ewhile cond cond s), ks) {{ Φ }}
+    ⊢ WP (Ewhile cond (Evalue vtrue) s, ks) {{ Φ }}.
   Proof. iIntros "Hnext". by wp_solve_pure. Qed.
 
-  Lemma wp_while_false cond s Φ:
+  Lemma wp_while_false cond s ks Φ:
     ▷ Φ Vvoid
-    ⊢ WP Ewhile cond (Evalue vfalse) s {{ Φ }}.
+    ⊢ WP (Ewhile cond (Evalue vfalse) s, ks) {{ Φ }}.
   Proof. iIntros "HΦ". wp_solve_pure. iApply wp_value=>//. Qed.
 
-  Lemma wp_while_inv I Q cond s:
+  Lemma wp_while_inv I Q cond s ks:
     is_jmp s = false → is_jmp cond = false →
-    □ (∀ Φ, (I ∗ (∀ v, ((⌜ v = vfalse ⌝ ∗ Q Vvoid) ∨ (⌜ v = vtrue ⌝ ∗ I)) -∗ Φ v) -∗ WP cond {{ Φ }})) ∗
-    □ (∀ Φ, (I ∗ (I -∗ Φ Vvoid)) -∗ WP s {{ Φ }}) ∗ I
-    ⊢ WP Ewhile cond cond s {{ Q }}.
+    □ (∀ Φ, (I ∗ (∀ v, ((⌜ v = vfalse ⌝ ∗ Q Vvoid) ∨ (⌜ v = vtrue ⌝ ∗ I)) -∗ Φ v) -∗ WP (cond, ks) {{ Φ }})) ∗
+    □ (∀ Φ, (I ∗ (I -∗ Φ Vvoid)) -∗ WP (s, ks) {{ Φ }}) ∗ I
+    ⊢ WP (Ewhile cond cond s, ks) {{ Q }}.
   Proof.
     iIntros (??) "(#Hcond & #Hs & HI)".
     iLöb as "IH".
@@ -469,24 +453,24 @@ Section rules.
       iApply "IH". by iNext.
   Qed.
 
-  Lemma wp_fst v1 v2 Φ:
+  Lemma wp_fst v1 v2 Φ ks:
     ▷ Φ v1
-    ⊢ WP Efst (Evalue (Vpair v1 v2)) {{ Φ }}.
+    ⊢ WP (Efst (Evalue (Vpair v1 v2)), ks) {{ Φ }}.
   Proof. iIntros "HΦ". wp_solve_pure. iApply wp_value=>//. Qed.
 
-  Lemma wp_snd v1 v2 Φ:
+  Lemma wp_snd v1 v2 Φ ks:
     ▷ Φ v2
-    ⊢ WP Esnd (Evalue (Vpair v1 v2)) {{ Φ }}.
+    ⊢ WP (Esnd (Evalue (Vpair v1 v2)), ks) {{ Φ }}.
   Proof. iIntros "HΦ". wp_solve_pure. iApply wp_value=>//. Qed.
 
-  Lemma wp_if_true e1 e2 Φ:
-    ▷ WP e1 {{ Φ }}
-    ⊢ WP (Eif (Evalue vtrue) e1 e2) {{ Φ }}.
+  Lemma wp_if_true e1 e2 Φ ks:
+    ▷ WP (e1, ks) {{ Φ }}
+    ⊢ WP (Eif (Evalue vtrue) e1 e2, ks) {{ Φ }}.
   Proof. iIntros "HΦ". wp_solve_pure. done. Qed.
 
-  Lemma wp_if_false e1 e2 Φ:
-    ▷ WP e2 {{ Φ }}
-    ⊢ WP (Eif (Evalue vfalse) e1 e2) {{ Φ }}.
+  Lemma wp_if_false e1 e2 Φ ks:
+    ▷ WP (e2, ks) {{ Φ }}
+    ⊢ WP (Eif (Evalue vfalse) e1 e2, ks) {{ Φ }}.
   Proof. iIntros "HΦ". wp_solve_pure. done. Qed.
 
   (* Freshness and memory allocation *)
@@ -542,14 +526,14 @@ Section rules.
       by iFrame.
   Qed.
 
-  Lemma wp_alloc E v t Φ:
+  Lemma wp_alloc E v t ks Φ:
     typeof v t →
     ▷ (∀ l, l ↦ v @ t -∗ Φ (Vptr l))
-    ⊢ WP Ealloc t (Evalue v) @ E {{ Φ }}.
+    ⊢ WP (Ealloc t (Evalue v), ks) @ E {{ Φ }}.
   Proof.
     iIntros (?) "HΦ".
     iApply wp_lift_atomic_step=>//.
-    iIntros (ks1 (σ1&Γ)) "[[Hσ1 HΓ] Hs]".
+    iIntros (ks1 (σ1&Γ)) "[Hσ1 HΓ]".
     iModIntro. iSplit.
     { iPureIntro. eexists _, _, _, [].
       apply CSestep. by apply alloc_fresh. }
@@ -560,10 +544,10 @@ Section rules.
     iApply "HΦ". by iFrame.
   Qed.
 
-  Lemma wp_let E x t v e e' Φ:
+  Lemma wp_let E x t v e e' Φ ks:
     instantiate_let x v t e = Some e' →
-    ▷ WP e' @ E {{ Φ }}
-    ⊢ WP Elet t x (Evalue v) e @ E {{ Φ }}.
+    ▷ WP (e', ks) @ E {{ Φ }}
+    ⊢ WP (Elet t x (Evalue v) e, ks) @ E {{ Φ }}.
   Proof.
     iIntros (?) "HΦ".
     iApply wp_lift_pure_step; first eauto.
@@ -572,7 +556,7 @@ Section rules.
       + inversion Hes=>//. simplify_eq.
         escape_false.
       + absurd_jstep Hjs.
-    - iNext. iIntros (e2 l1 l2 σ1 σ2 efs Hcs). subst.
+    - iNext. iIntros (e2 l2 σ1 σ2 efs Hcs). subst.
       inversion_cstep_as Hes Hjs.
       + inversion Hes=>//; simplify_eq=>//.
         * iSplitL; last by rewrite big_sepL_nil. done.
@@ -608,22 +592,22 @@ Section rules.
       as %[Hl %text_singleton_included]%auth_valid_discrete_2.
   Qed.
  
-  Lemma wp_fork E t f vs params e e' Φ :
+  Lemma wp_fork E t f vs params e e' Φ ks:
     let_params vs params e = Some e' →
-    text_interp f (Function t params e) ∗ ▷ Φ Vvoid ∗ ▷ (own_stack [] -∗ WP e' {{ _, True }})
-    ⊢ WP Efork t f (map Evalue vs) @ E {{ Φ }}.
+    text_interp f (Function t params e) ∗ ▷ Φ Vvoid ∗ ▷ (WP (e', []) {{ _, True }})
+    ⊢ WP (Efork t f (map Evalue vs), ks) @ E {{ Φ }}.
   Proof.
     iIntros (?) "(Hf & HΦ & He)".
     iApply wp_lift_step=>//.
-    iIntros (ks1 (σ1&Γ)) "[[Hσ1 HΓ] Hs]".
+    iIntros (σ1) "[Hσ1 HΓ]".
     iMod (fupd_intro_mask' _ ∅) as "Hclose"; first set_solver.
     iDestruct (lookup_text with "[HΓ Hf]") as "%"; first iFrame=>//.
     simpl in *. iModIntro. iSplit.
-    { iPureIntro. eexists (Evalue Vvoid), _, _, [e']. simpl.
-      destruct σ1. apply CSestep. by econstructor. }
-    iNext. iIntros (?????Hcs).
+    { iPureIntro. eexists (Evalue Vvoid), ks, σ1, [e']. simpl.
+      destruct σ1. simpl in *. apply CSestep. by econstructor. }
+    iNext. iIntros (????Hcs).
     iMod "Hclose". inversion_cstep_as Hes Hjs.
-    - iModIntro. iFrame. simpl in *.
+    - iModIntro. iFrame. simpl in *. destruct a. simpl in *.
       inversion Hes=>//; subst.
       + iFrame. iSplitR "He".
         { iApply wp_value=>//. }
@@ -637,29 +621,27 @@ Section rules.
   Lemma wp_call {E ks} k vs params e e' f retty Φ:
     let_params vs params e = Some e' →
     text_interp f (Function retty params e) ∗
-    own_stack ks ∗
-    ▷ (own_stack (k::ks) -∗ WP e' @ E {{ Φ }})
-    ⊢ WP fill_ectxs (Ecall retty f (map Evalue vs)) k @ E {{ Φ }}.
+    ▷ WP (e', k::ks) @ E {{ Φ }}
+    ⊢ WP (fill_ectxs (Ecall retty f (map Evalue vs)) k, ks) @ E {{ Φ }}.
   Proof.
-    iIntros (Hls) "[Hf [Hstk HΦ]]".
+    iIntros (Hls) "[Hf HΦ]".
     iApply wp_lift_step=>//.
     { apply fill_ectxs_not_val. done. }
-    iIntros (ks1 (σ1&Γ)) "[[Hσ1 HΓ] Hs]".
+    iIntros (σ1) "[Hσ1 HΓ]".
     iMod (fupd_intro_mask' _ ∅) as "Hclose"; first set_solver.
     iDestruct (lookup_text with "[HΓ Hf]") as "%"; first iFrame=>//.
     simpl in *. iModIntro. iSplit.
-    { iPureIntro. eexists _, _, _, [].
+    { iPureIntro. eexists _, _, _, []. destruct σ1. simpl in *.
       apply CSjstep. eapply JScall=>//. }
-    iNext. iIntros (e2 l2 σ2 efs Hcs).
+    iNext. iIntros (e2 σ2 efs Hcs).
     iMod "Hclose". inversion_cstep_as Hes Hjs.
     { apply fill_estep_false in Hes=>//. }
     inversion_jstep_as Heq.
     + fill_enf_neq.
     + apply cont_inj in Heq=>//; auto.
       destruct Heq as [Heq ?]. inversion Heq. subst.
-      iFrame. iDestruct (own_pair_agree with "[Hs Hstk]") as "%"; first iFrame.
-      subst. iMod (stack_push with "[Hs Hstk]") as "(Hs & Hstk & %)"; first iFrame.
-      iFrame. assert (vs0 = vs) as ?.
+      iFrame. destruct e2. simpl in *. subst.
+      assert (vs0 = vs) as ?.
       { eapply map_inj=>//. simpl. by inversion 1. }
       subst. clear Heq. simplify_eq.
       iSplitL; first by iApply "HΦ".
