theories/tests/spawn.v
@@ -19,20 +19,20 @@ Section test.
     Ecall Tvoid f_release [Evalue l].
 
   Lemma add_safe ks:
-    own_stack ks ∗ is_lock N γ l R ∗
+    is_lock N γ l R ∗
     text_interp f_release (Function Tvoid [(x, tylock)] release) ∗
     text_interp f_acquire (Function Tvoid [(x, tylock)] acquire)
-    ⊢ WP add {{ _, True }}.
+    ⊢ WP (add, ks) {{ _, True }}.
   Proof.
-    iIntros "(Hs & #Hlk & H1 & H2)". unfold add.
+    iIntros "(#Hlk & H1 & H2)". unfold add.
     wp_unfill (Ecall _ _ _).
     iApply acquire_spec. iFrame. iFrame "#".
-    iIntros "Hlked HR Hks".
+    iIntros "Hlked HR".
     iDestruct "HR" as (?) "Hvx".
     wp_skip. wp_load. wp_op. wp_assign.
     iApply (release_spec []). iFrame "Hlk".
     iFrame. iSplitL "Hvx"; first by iExists _.
-    iIntros "Hks". iApply wp_value=>//.
+    iApply wp_value=>//.
   Qed.
 
   (* It is just DRF property -- though we can have a stronger spec
@@ -42,12 +42,12 @@ Section test.
     Efork Tvoid f_add [] ;;
     Efork Tvoid f_add [].
 
-  Lemma spawn_spec:
+  Lemma spawn_spec ks:
     is_lock N γ l R ∗
     text_interp f_release (Function Tvoid [(x, tylock)] release) ∗
     text_interp f_acquire (Function Tvoid [(x, tylock)] acquire) ∗
     text_interp f_add (Function Tvoid [] add)
-    ⊢ WP spawn {{ _, True }}.
+    ⊢ WP (spawn, ks) {{ _, True }}.
   Proof.
     iIntros "(#Hlk & Hf1 & Hf2 & Hf3)".
     unfold spawn. iApply wp_seq=>//.
@@ -57,8 +57,8 @@ Section test.
     iDestruct (text_interp_dup with "Hf2") as "[Hf2 Hf2']".
     iSplitL "Hf1 Hf2 Hf3".
     - wp_skip. iApply (wp_fork _ _ _ []); last iFrame; first done.
-      iNext. iSplit=>//. iIntros "?". iApply add_safe. by iFrame.
-    - iIntros "?". iApply add_safe. by iFrame.
+      iNext. iSplit=>//. iApply add_safe. by iFrame.
+    - iApply add_safe. by iFrame.
   Qed.
 
 End test.
