theories/tests/swap.v
@@ -17,9 +17,9 @@ Section example.
   Definition swap' t  (l1 l2: addr) :=
     instantiate_let a1 l1 t (swap t) ≫= instantiate_let a2 l2 t.
   
-  Lemma swap_spec' t swap_e l1 l2 v1 v2 :
+  Lemma swap_spec' t swap_e l1 l2 v1 v2 ks:
     swap' t l1 l2 = Some swap_e →
-    {{{ l1 ↦ v1 @ t ∗ l2 ↦ v2 @ t }}} swap_e {{{ RET void ; l1 ↦ v2 @ t ∗ l2 ↦ v1 @ t }}}.
+    {{{ l1 ↦ v1 @ t ∗ l2 ↦ v2 @ t }}} (swap_e, ks) {{{ RET void ; l1 ↦ v2 @ t ∗ l2 ↦ v1 @ t }}}.
   Proof.
     iIntros (H0 ?) "[??] HΦ". inversion H0. extract_types.
     wp_alloc lx as "Hlx". wp_run. iApply ("HΦ" with "[-]"). iFrame.
